Examples.v
@@ -38,44 +38,42 @@ From Elo Require Import Core.
 
 Definition example1 : tm := <{
   let "m1" : x&w&Nat = new (new (nat 3) : w&Nat) : x&w&Nat in
-  let "m2" : x&w&Nat = new (new (nat 5) : w&Nat) : x&w&Nat in
-  spawn (
-    acq (var "m1") "x" (
-      let "result" : Nat = *(var "x") in (
-        (var "x") := (nat 6);
-        (var "result")
+  let "m2" : x&w&Nat = new (new (nat 5) : w&Nat) : x&w&Nat in (
+    spawn (
+      acq (var "m1") "x" (
+        let "result" : Nat = *(var "x") in (
+          (var "x") := (nat 6);
+          (var "result")
+        )
       )
-    )
-  );
-  spawn (
-    acq (var "m2") "y" (
-      let "result" : Nat = *(var "y") in (
-        (var "y") := (nat 10);
-        (var "result")
+    );
+    spawn (
+      acq (var "m2") "y" (
+        let "result" : Nat = *(var "y") in (
+          (var "y") := (nat 10);
+          (var "result")
+        )
       )
-    )
-  );
-  (nat 20)
+    );
+    (nat 20)
+  )
 }>.
 
 Ltac solve_ty :=
   repeat match goal with
-  | |- _ |-- <{unit        }> is _ => eapply T_unit
-  | |- _ |-- <{nat _       }> is _ => eapply T_nat
-  | |- _ |-- <{_; _        }> is _ => eapply T_seq
-  | |- _ |-- <{var _       }> is _ => eapply T_var
-  | |- _ |-- <{fn _ _ _    }> is _ => eapply T_fun
-  | |- _ |-- <{call _ _    }> is _ => eapply T_call
-  | |- _ |-- <{new _ : r&?T}> is _ => eapply T_newR
-  | |- _ |-- <{new _ : x&?T}> is _ => eapply T_newX
-  | |- _ |-- <{new _ : w&?T}> is _ => eapply T_newW
-  (*
-  | T_loadR : forall Gamma t T, Gamma |-- <{*t}> is `Safe T`
-  | T_loadW : forall Gamma t T, Gamma |-- <{*t}> is T
-  *)
-  | |- _ |-- <{_ := _      }> is _ => eapply T_asg
-  | |- _ |-- <{acq _ _ _   }> is _ => eapply T_acq
-  | |- _ |-- <{spawn _     }> is _ => eapply T_spawn
+  | |- _ |-- <{unit                  }> is _ => eapply T_unit
+  | |- _ |-- <{nat _                 }> is _ => eapply T_nat
+  | |- _ |-- <{_; _                  }> is _ => eapply T_seq
+  | |- _ |-- <{if _ then _ else _ end}> is _ => eapply T_if
+  | |- _ |-- <{var _                 }> is _ => eapply T_var
+  | |- _ |-- <{fn _ _ _              }> is _ => eapply T_fun
+  | |- _ |-- <{call _ _              }> is _ => eapply T_call
+  | |- _ |-- <{new _ : r&?T          }> is _ => eapply T_newR
+  | |- _ |-- <{new _ : x&?T          }> is _ => eapply T_newX
+  | |- _ |-- <{new _ : w&?T          }> is _ => eapply T_newW
+  | |- _ |-- <{_ := _                }> is _ => eapply T_asg
+  | |- _ |-- <{acq _ _ _             }> is _ => eapply T_acq
+  | |- _ |-- <{spawn _               }> is _ => eapply T_spawn
   end.
 
 Lemma example1_is_well_typed :
@@ -105,9 +103,9 @@ Lemma example1_reduces_correctly : forall m ths,
     <{nat 10}> ::
     <{nat 20}> ::
     nil) ->
-  exists tc, base_m / (base_t example1) ~~[tc]~~>* m / ths.
+  exists tc, nil / (base example1) ~~[tc]~~>* m / ths.
 Proof.
-  unfold base_m, base_t. intros. eexists.
+  unfold base. intros. eexists.
   eapply multistep_trans.
 Abort.
 
