HasVar.v
@@ -6,57 +6,64 @@ From Elo Require Import Core.
 
 Inductive has_var (x : id) : tm  -> Prop :=
   | hasvar_seq1  : forall t1 t2,    has_var x t1 ->
-                                    has_var x <{t1; t2       }>
+                                    has_var x <{t1; t2                   }>
   | hasvar_seq2  : forall t1 t2,    has_var x t2 ->
-                                    has_var x <{t1; t2       }>
-  | hasvar_var   :                  has_var x <{var x        }>
+                                    has_var x <{t1; t2                   }>
+  | hasvar_if1   : forall t1 t2 t3, has_var x t1 ->
+                                    has_var x <{if t1 then t2 else t3 end}>
+  | hasvar_if2   : forall t1 t2 t3, has_var x t2 ->
+                                    has_var x <{if t1 then t2 else t3 end}>
+  | hasvar_if3   : forall t1 t2 t3, has_var x t3 ->
+                                    has_var x <{if t1 then t2 else t3 end}>
+  | hasvar_var   :                  has_var x <{var x                    }>
   | hasvar_fun   : forall x' Tx t,  x <> x'      ->
                                     has_var x t  ->
-                                    has_var x <{fn x' Tx t   }>
+                                    has_var x <{fn x' Tx t               }>
   | hasvar_call1 : forall t1 t2,    has_var x t1 ->
-                                    has_var x <{call t1 t2   }>
+                                    has_var x <{call t1 t2               }>
   | hasvar_call2 : forall t1 t2,    has_var x t2 ->
-                                    has_var x <{call t1 t2   }>
+                                    has_var x <{call t1 t2               }>
   | hasvar_new   : forall t T,      has_var x t  ->
-                                    has_var x <{new t : T    }>
+                                    has_var x <{new t : T                }>
   | hasvar_init  : forall ad t T,   has_var x t  ->
-                                    has_var x <{init ad t : T}>
+                                    has_var x <{init ad t : T            }>
   | hasvar_load  : forall t,        has_var x t  ->
-                                    has_var x <{*t           }>
+                                    has_var x <{*t                       }>
   | hasvar_asg1  : forall t1 t2,    has_var x t1 ->
-                                    has_var x <{t1 := t2     }>
+                                    has_var x <{t1 := t2                 }>
   | hasvar_asg2  : forall t1 t2,    has_var x t2 ->
-                                    has_var x <{t1 := t2     }>
+                                    has_var x <{t1 := t2                 }>
   | hasvar_acq1  : forall t1 x' t2, has_var x t1 ->
-                                    has_var x <{acq t1 x' t2 }>
+                                    has_var x <{acq t1 x' t2             }>
   | hasvar_acq2  : forall t1 x' t2, x <> x'      ->
                                     has_var x t2 ->
-                                    has_var x <{acq t1 x' t2 }>
+                                    has_var x <{acq t1 x' t2             }>
   | hasvar_cr    : forall ad t,     has_var x t  ->
-                                    has_var x <{cr ad t      }>
+                                    has_var x <{cr ad t                  }>
   | hasvar_spawn : forall t,        has_var x t  ->
-                                    has_var x <{spawn t      }>
+                                    has_var x <{spawn t                  }>
   .
 
 (* inversion --------------------------------------------------------------- *)
 
 Local Ltac _hasvar tt :=
   match goal with
-  | H : has_var _  <{unit          }> |- _ => invc H
-  | H : has_var _  <{nat _         }> |- _ => invc H
-  | H : has_var _  <{_; _          }> |- _ => tt H
-  | H : has_var ?x <{var ?x        }> |- _ => clear H
-  | H : has_var _  <{var _         }> |- _ => tt H
-  | H : has_var _  <{fn _ _ _      }> |- _ => tt H
-  | H : has_var _  <{call _ _      }> |- _ => tt H
-  | H : has_var _  <{&_ : _        }> |- _ => invc H
-  | H : has_var _  <{new _ : _     }> |- _ => tt H
-  | H : has_var _  <{init _ _ : _  }> |- _ => tt H
-  | H : has_var _  <{* _           }> |- _ => tt H
-  | H : has_var _  <{_ := _        }> |- _ => tt H
-  | H : has_var _  <{acq _ _ _     }> |- _ => tt H
-  | H : has_var _  <{cr _ _        }> |- _ => tt H
-  | H : has_var _  <{spawn _       }> |- _ => tt H
+  | H : has_var _  <{unit                  }> |- _ => invc H
+  | H : has_var _  <{nat _                 }> |- _ => invc H
+  | H : has_var _  <{_; _                  }> |- _ => tt H
+  | H : has_var _  <{if _ then _ else _ end}> |- _ => tt H
+  | H : has_var ?x <{var ?x                }> |- _ => clear H
+  | H : has_var _  <{var _                 }> |- _ => tt H
+  | H : has_var _  <{fn _ _ _              }> |- _ => tt H
+  | H : has_var _  <{call _ _              }> |- _ => tt H
+  | H : has_var _  <{&_ : _                }> |- _ => invc H
+  | H : has_var _  <{new _ : _             }> |- _ => tt H
+  | H : has_var _  <{init _ _ : _          }> |- _ => tt H
+  | H : has_var _  <{* _                   }> |- _ => tt H
+  | H : has_var _  <{_ := _                }> |- _ => tt H
+  | H : has_var _  <{acq _ _ _             }> |- _ => tt H
+  | H : has_var _  <{cr _ _                }> |- _ => tt H
+  | H : has_var _  <{spawn _               }> |- _ => tt H
   end.
 
 Ltac inv_hasvar  := _hasvar inv.
@@ -68,7 +75,7 @@ Corollary hasvar_dec : forall x t,
   Decidable.decidable (has_var x t).
 Proof.
   unfold Decidable.decidable. intros. induction t;
-  try (destruct IHt || destruct IHt1, IHt2);
+  try (destruct IHt1, IHt2, IHt3 || destruct IHt1, IHt2 || destruct IHt);
   try match goal with x1: id, x2: id |- _ => str_eq_dec x1 x2 end;
   auto using has_var;
   right; intros ?; invc_hasvar; auto.
@@ -82,10 +89,11 @@ Lemma hasvar_subst : forall x t tx,
 Proof.
   intros * Hnhv **. induction t; simpl; trivial;
   try destruct _str_eq_dec; subst; trivial;
-  solve [ rewrite <- IHt; auto using has_var
-        | rewrite <- IHt1; try rewrite <- IHt2; auto using has_var
-        | exfalso; auto using has_var
-        ].
+  try (rewrite <- IHt;  auto using has_var);
+  try (rewrite <- IHt1; auto using has_var);
+  try (rewrite <- IHt2; auto using has_var);
+  try (rewrite <- IHt3; auto using has_var).
+  exfalso. auto using has_var.
 Qed.
 
 Lemma hasvar_type_contradiction : forall Gamma x t T,
