NoCR.v
@@ -5,56 +5,61 @@ From Elo Require Import Core.
 (* ------------------------------------------------------------------------- *)
 
 Inductive no_cr (ad : addr) : tm -> Prop :=
-  | nocr_unit  :                 no_cr ad <{unit          }>
-  | nocr_nat   : forall n,       no_cr ad <{nat n         }>
-  | nocr_seq   : forall t1 t2,   no_cr ad t1 ->
-                                 no_cr ad t2 ->
-                                 no_cr ad <{t1; t2        }>
-  | nocr_var   : forall x,       no_cr ad <{var x         }>
-  | nocr_fun   : forall x Tx t,  no_cr ad t  ->
-                                 no_cr ad <{fn x Tx t     }>
-  | nocr_call  : forall t1 t2,   no_cr ad t1 ->
-                                 no_cr ad t2 ->
-                                 no_cr ad <{call t1 t2    }>
-  | nocr_ref   : forall ad' T,   no_cr ad <{&ad' : T      }>
-  | nocr_new   : forall t T,     no_cr ad t  ->
-                                 no_cr ad <{new t : T     }>
-  | nocr_init  : forall ad' t T, no_cr ad t  ->
-                                 no_cr ad <{init ad' t : T}>
-  | nocr_load  : forall t,       no_cr ad t  ->
-                                 no_cr ad <{*t            }>
-  | nocr_asg   : forall t1 t2,   no_cr ad t1 ->
-                                 no_cr ad t2 ->
-                                 no_cr ad <{t1 := t2      }>
-  | nocr_acq   : forall t1 x t2, no_cr ad t1 ->
-                                 no_cr ad t2 ->
-                                 no_cr ad <{acq t1 x t2   }>
-  | nocr_cr    : forall ad' t,   ad <> ad'   ->
-                                 no_cr ad t  ->
-                                 no_cr ad <{cr ad' t      }>
-  | nocr_spawn : forall t,       no_cr ad t  ->
-                                 no_cr ad <{spawn t       }>
+  | nocr_unit  :                  no_cr ad <{unit                     }>
+  | nocr_nat   : forall n,        no_cr ad <{nat n                    }>
+  | nocr_seq   : forall t1 t2,    no_cr ad t1 ->
+                                  no_cr ad t2 ->
+                                  no_cr ad <{t1; t2                   }>
+  | nocr_if    : forall t1 t2 t3, no_cr ad t1 ->
+                                  no_cr ad t2 ->
+                                  no_cr ad t3 ->
+                                  no_cr ad <{if t1 then t2 else t3 end}>
+  | nocr_var   : forall x,        no_cr ad <{var x                    }>
+  | nocr_fun   : forall x Tx t,   no_cr ad t  ->
+                                  no_cr ad <{fn x Tx t                }>
+  | nocr_call  : forall t1 t2,    no_cr ad t1 ->
+                                  no_cr ad t2 ->
+                                  no_cr ad <{call t1 t2               }>
+  | nocr_ref   : forall ad' T,    no_cr ad <{&ad' : T                 }>
+  | nocr_new   : forall t T,      no_cr ad t  ->
+                                  no_cr ad <{new t : T                }>
+  | nocr_init  : forall ad' t T,  no_cr ad t  ->
+                                  no_cr ad <{init ad' t : T           }>
+  | nocr_load  : forall t,        no_cr ad t  ->
+                                  no_cr ad <{*t                       }>
+  | nocr_asg   : forall t1 t2,    no_cr ad t1 ->
+                                  no_cr ad t2 ->
+                                  no_cr ad <{t1 := t2                 }>
+  | nocr_acq   : forall t1 x t2,  no_cr ad t1 ->
+                                  no_cr ad t2 ->
+                                  no_cr ad <{acq t1 x t2              }>
+  | nocr_cr    : forall ad' t,    ad <> ad'   ->
+                                  no_cr ad t  ->
+                                  no_cr ad <{cr ad' t                 }>
+  | nocr_spawn : forall t,        no_cr ad t  ->
+                                  no_cr ad <{spawn t                  }>
   .
 
 (* inversion --------------------------------------------------------------- *)
 
 Local Ltac _nocr tt :=
   match goal with
-  | H : no_cr _   <{unit        }> |- _ => clear H
-  | H : no_cr _   <{nat _       }> |- _ => clear H
-  | H : no_cr _   <{_; _        }> |- _ => tt H
-  | H : no_cr _   <{var _       }> |- _ => clear H
-  | H : no_cr _   <{fn _ _ _    }> |- _ => tt H
-  | H : no_cr _   <{call _ _    }> |- _ => tt H
-  | H : no_cr _   <{&_ : _      }> |- _ => clear H
-  | H : no_cr _   <{new _ : _   }> |- _ => tt H
-  | H : no_cr _   <{init _ _ : _}> |- _ => tt H
-  | H : no_cr _   <{* _         }> |- _ => tt H
-  | H : no_cr _   <{_ := _      }> |- _ => tt H
-  | H : no_cr _   <{acq _ _ _   }> |- _ => tt H
-  | H : no_cr ?ad <{cr ?ad _    }> |- _ => invc H; auto
-  | H : no_cr _   <{cr _ _      }> |- _ => tt H
-  | H : no_cr _   <{spawn _     }> |- _ => tt H
+  | H : no_cr _   <{unit                  }> |- _ => clear H
+  | H : no_cr _   <{nat _                 }> |- _ => clear H
+  | H : no_cr _   <{_; _                  }> |- _ => tt H
+  | H : no_cr _   <{if _ then _ else _ end}> |- _ => tt H
+  | H : no_cr _   <{var _                 }> |- _ => clear H
+  | H : no_cr _   <{fn _ _ _              }> |- _ => tt H
+  | H : no_cr _   <{call _ _              }> |- _ => tt H
+  | H : no_cr _   <{&_ : _                }> |- _ => clear H
+  | H : no_cr _   <{new _ : _             }> |- _ => tt H
+  | H : no_cr _   <{init _ _ : _          }> |- _ => tt H
+  | H : no_cr _   <{* _                   }> |- _ => tt H
+  | H : no_cr _   <{_ := _                }> |- _ => tt H
+  | H : no_cr _   <{acq _ _ _             }> |- _ => tt H
+  | H : no_cr ?ad <{cr ?ad _              }> |- _ => invc H; auto
+  | H : no_cr _   <{cr _ _                }> |- _ => tt H
+  | H : no_cr _   <{spawn _               }> |- _ => tt H
   end.
 
 Ltac inv_nocr  := _nocr inv.
@@ -67,7 +72,8 @@ Lemma nocr_dec : forall ad t,
 Proof.
   unfold Decidable.decidable. unfold not. intros.
   induction t; auto using no_cr;
-  (destruct IHt || destruct IHt1, IHt2); auto using no_cr;
+  (destruct IHt1, IHt2, IHt3 || destruct IHt1, IHt2 || destruct IHt);
+  auto using no_cr;
   try solve [right; intros; invc_nocr; auto].
   match goal with ad1 : addr, ad2 : addr |- _ => nat_eq_dec ad1 ad2 end;
   auto using no_cr. right. intros. invc_nocr.
@@ -176,10 +182,14 @@ Definition no_crs (t : tm) := forall ad, no_cr ad t.
 (* inversion --------------------------------------------------------------- *)
 
 Local Ltac solve_inv_nocrs :=
-  unfold no_crs; intros * H; try split; intros; spec; invc_nocr; auto.
+  unfold no_crs; intros * H; repeat split; intros; spec; invc_nocr; auto.
 
 Local Lemma inv_nocrs_seq : forall t1 t2,
   no_crs <{t1; t2}> -> no_crs t1 /\ no_crs t2.
+Proof. solve_inv_nocrs. Qed.
+
+Local Lemma inv_nocrs_if : forall t1 t2 t3,
+  no_crs (tm_if t1 t2 t3) -> no_crs t1 /\ no_crs t2 /\ no_crs t3.
 Proof. solve_inv_nocrs. Qed.
 
 Local Lemma inv_nocrs_fun : forall x Tx t,
@@ -223,6 +233,7 @@ Ltac invc_nocrs :=
   | H : no_crs <{unit        }> |- _ => clear H
   | H : no_crs <{nat _       }> |- _ => clear H
   | H : no_crs <{_; _        }> |- _ => eapply inv_nocrs_seq   in H as [? ?]
+  | H : no_crs (tm_if _ _ _  )  |- _ => eapply inv_nocrs_if    in H as [? [? ?]]
   | H : no_crs <{var _       }> |- _ => clear H
   | H : no_crs <{fn _ _ _    }> |- _ => eapply inv_nocrs_fun   in H
   | H : no_crs <{call _ _    }> |- _ => eapply inv_nocrs_call  in H as [? ?]
