Kappa.v
@@ -6,75 +6,107 @@ From Elo Require Import SemExt.
 (* kappa                                                                     *)
 (* ------------------------------------------------------------------------- *)
 
-Lemma gcr_rewrite_seq_t1 : forall t1 t2 R,
-  ~ value t1 ->
-  gcr <{t1; t2}> R = gcr t1 R.
-Proof.
-  intros * H. simpl. destruct t1; auto; exfalso; auto using value.
-Qed.
-
-Lemma gcr_rewrite_seq_t2 : forall t1 t2 R,
+Lemma kappa_seq__value : forall t1 t2 R,
   value t1 ->
   gcr <{t1; t2}> R = gcr t2 R.
 Proof.
   intros * H. simpl. destruct t1; auto; invc H.
 Qed.
 
-Lemma gcr_rewrite_call_t1 : forall t1 t2 R,
+Lemma kappa_seq__not_value : forall t1 t2 R,
   ~ value t1 ->
-  gcr <{call t1 t2}> R = gcr t1 R.
+  gcr <{t1; t2}> R = gcr t1 R.
 Proof.
   intros * H. simpl. destruct t1; auto; exfalso; auto using value.
 Qed.
 
-Lemma gcr_rewrite_call_t2 : forall t1 t2 R,
+(* ------------------------------------------------------------------------- *)
+
+Lemma kappa_if__value : forall t1 t2 t3 R,
+  value t1 ->
+  gcr <{if t1 then t2 else t3 end}> R = R.
+Proof.
+  intros * H. simpl. destruct t1; auto; invc H.
+Qed.
+
+Lemma kappa_if__not_value : forall t1 t2 t3 R,
+  ~ value t1 ->
+  gcr <{if t1 then t2 else t3 end}> R = gcr t1 R.
+Proof.
+  intros * H. simpl. destruct t1; auto; exfalso; auto using value.
+Qed.
+
+(* ------------------------------------------------------------------------- *)
+
+Lemma kappa_call__value : forall t1 t2 R,
   value t1 ->
   gcr <{call t1 t2}> R = gcr t2 R.
 Proof.
   intros * H. simpl. destruct t1; auto; invc H.
 Qed.
 
-Lemma gcr_rewrite_initX : forall ad t T R,
-  gcr <{init ad t : x&T}> R = gcr t (R_ad ad).
-Proof. trivial. Qed.
-
-Lemma gcr_rewrite_initW : forall ad t T R,
-  gcr <{init ad t : w&T}> R = gcr t R.
-Proof. trivial. Qed.
-
-Lemma gcr_rewrite_asg_t1 : forall t1 t2 R,
+Lemma kappa_call__not_value : forall t1 t2 R,
   ~ value t1 ->
-  gcr <{t1 := t2}> R = gcr t1 R.
+  gcr <{call t1 t2}> R = gcr t1 R.
 Proof.
   intros * H. simpl. destruct t1; auto; exfalso; auto using value.
 Qed.
 
-Lemma gcr_rewrite_asg_t2 : forall t1 t2 R,
+(* ------------------------------------------------------------------------- *)
+
+Lemma kappa_initX : forall ad t T R,
+  gcr <{init ad t : x&T}> R = gcr t (R_ad ad).
+Proof. trivial. Qed.
+
+Lemma kappa_initW : forall ad t T R,
+  gcr <{init ad t : w&T}> R = gcr t R.
+Proof. trivial. Qed.
+
+(* ------------------------------------------------------------------------- *)
+
+Lemma kappa_asg__value : forall t1 t2 R,
   value t1 ->
   gcr <{t1 := t2}> R = gcr t2 R.
 Proof.
   intros * H. simpl. destruct t1; auto; invc H.
 Qed.
 
+Lemma kappa_asg__not_value : forall t1 t2 R,
+  ~ value t1 ->
+  gcr <{t1 := t2}> R = gcr t1 R.
+Proof.
+  intros * H. simpl. destruct t1; auto; exfalso; auto using value.
+Qed.
+
+(* ------------------------------------------------------------------------- *)
+
 (* gcr (get-current-region) simplification *)
 Ltac kappa :=
  repeat match goal with
- | H : context C [ gcr <{?t1; ?t2    }> ?R ], H' : ~ value ?t1 |- _ =>
-   rewrite (gcr_rewrite_seq_t1 t1 t2 R H') in H
- | H : context C [ gcr <{?t1; ?t2    }> ?R ], H' : value   ?t1 |- _ =>
-   rewrite (gcr_rewrite_seq_t2 t1 t2 R H') in H
- | H : context C [ gcr <{call ?t1 ?t2}> ?R ], H' : ~ value ?t1 |- _ =>
-   rewrite (gcr_rewrite_call_t1 t1 t2 R H') in H
- | H : context C [ gcr <{call ?t1 ?t2}> ?R ], H' : value   ?t1 |- _ =>
-   rewrite (gcr_rewrite_call_t2 t1 t2 R H') in H
- | H : context C [ gcr <{?t1 := ?t2  }> ?R ], H' : ~ value ?t1 |- _ =>
-   rewrite (gcr_rewrite_asg_t1 t1 t2 R H') in H
- | H : context C [ gcr <{?t1 := ?t2  }> ?R ], H' : value   ?t1 |- _ =>
-   rewrite (gcr_rewrite_asg_t2 t1 t2 R H') in H
+ | H : context C [ gcr <{?t1; ?t2    }> ?R ],    H' : value   ?t1 |- _ =>
+   rewrite (kappa_seq__value      t1 t2 R H')    in H
+ | H : context C [ gcr <{?t1; ?t2    }> ?R ],    H' : ~ value ?t1 |- _ =>
+   rewrite (kappa_seq__not_value  t1 t2 R H')    in H
+
+ | H : context C [ gcr (tm_if ?t1 ?t2 ?t3) ?R ], H' : value ?t1 |- _   =>
+   rewrite (kappa_if__value       t1 t2 t3 R H') in H
+ | H : context C [ gcr (tm_if ?t1 ?t2 ?t3) ?R ], H' : ~ value ?t1 |- _ =>
+   rewrite (kappa_if__not_value   t1 t2 t3 R H') in H
+
+ | H : context C [ gcr <{call ?t1 ?t2}> ?R ],    H' : value   ?t1 |- _ =>
+   rewrite (kappa_call__value     t1 t2 R H')    in H
+ | H : context C [ gcr <{call ?t1 ?t2}> ?R ],    H' : ~ value ?t1 |- _ =>
+   rewrite (kappa_call__not_value t1 t2 R H')    in H
+
+ | H : context C [ gcr <{?t1 := ?t2  }> ?R ],    H' : value   ?t1 |- _ =>
+   rewrite (kappa_asg__value      t1 t2 R H')    in H
+ | H : context C [ gcr <{?t1 := ?t2  }> ?R ],    H' : ~ value ?t1 |- _ =>
+   rewrite (kappa_asg__not_value  t1 t2 R H')    in H
 
  | H : context C [gcr <{unit                }> _] |- _ => simpl in H
  | H : context C [gcr <{nat _               }> _] |- _ => simpl in H
  | H : context C [gcr <{?t; _               }> _] |- _ => destruct (value_dec t)
+ | H : context C [gcr (tm_if ?t _ _         )  _] |- _ => destruct (value_dec t)
  | H : context C [gcr <{var _               }> _] |- _ => simpl in H
  | H : context C [gcr <{fn _ _ _            }> _] |- _ => simpl in H
  | H : context C [gcr <{call ?t _           }> _] |- _ => destruct (value_dec t)
@@ -94,22 +126,30 @@ Ltac kappa :=
  | H : context C [gcr <{cr _ _              }> _] |- _ => simpl in H
  | H : context C [gcr <{spawn _             }> _] |- _ => simpl in H
 
- | H' : ~ value ?t1 |- context C [ gcr <{?t1; ?t2    }> ?R ] =>
-   rewrite (gcr_rewrite_seq_t1 t1 t2 R H')
- | H' : value   ?t1 |- context C [ gcr <{?t1; ?t2    }> ?R ] =>
-   rewrite (gcr_rewrite_seq_t2 t1 t2 R H')
- | H' : ~ value ?t1 |- context C [ gcr <{call ?t1 ?t2}> ?R ] =>
-   rewrite (gcr_rewrite_call_t1 t1 t2 R H')
- | H' : value   ?t1 |- context C [ gcr <{call ?t1 ?t2}> ?R ] =>
-   rewrite (gcr_rewrite_call_t2 t1 t2 R H')
- | H' : ~ value ?t1 |- context C [ gcr <{?t1 := ?t2  }> ?R ] =>
-   rewrite (gcr_rewrite_asg_t1 t1 t2 R H')
- | H' : value   ?t1 |- context C [ gcr <{?t1 := ?t2  }> ?R ] =>
-   rewrite (gcr_rewrite_asg_t2 t1 t2 R H')
+ | H' : value   ?t1 |- context C [ gcr <{?t1; ?t2       }> ?R ] =>
+   rewrite (kappa_seq__value      t1 t2 R H')
+ | H' : ~ value ?t1 |- context C [ gcr <{?t1; ?t2       }> ?R ] =>
+   rewrite (kappa_seq__not_value  t1 t2 R H')
+
+ | H' : value   ?t1 |- context C [ gcr (tm_if ?t1 ?t2 ?t3) ?R ] =>
+   rewrite (kappa_if__value       t1 t2 t3 R H')
+ | H' : ~ value ?t1 |- context C [ gcr (tm_if ?t1 ?t2 ?t3) ?R ] =>
+   rewrite (kappa_if__not_value   t1 t2 t3 R H')
+
+ | H' : value   ?t1 |- context C [ gcr <{call ?t1 ?t2   }> ?R ] =>
+   rewrite (kappa_call__value     t1 t2 R H')
+ | H' : ~ value ?t1 |- context C [ gcr <{call ?t1 ?t2   }> ?R ] =>
+   rewrite (kappa_call__not_value t1 t2 R H')
+
+ | H' : value   ?t1 |- context C [ gcr <{?t1 := ?t2     }> ?R ] =>
+   rewrite (kappa_asg__value      t1 t2 R H')
+ | H' : ~ value ?t1 |- context C [ gcr <{?t1 := ?t2     }> ?R ] =>
+   rewrite (kappa_asg__not_value  t1 t2 R H')
 
  | |- context C [gcr <{unit                }> _] => simpl
  | |- context C [gcr <{nat _               }> _] => simpl
  | |- context C [gcr <{?t; _               }> _] => destruct (value_dec t)
+ | |- context C [gcr (tm_if ?t _ _         )  _] => destruct (value_dec t)
  | |- context C [gcr <{var _               }> _] => simpl
  | |- context C [gcr <{fn _ _ _            }> _] => simpl
  | |- context C [gcr <{call ?t _           }> _] => destruct (value_dec t)
