MemoryRegions.v
@@ -15,7 +15,7 @@ Theorem mreg_preservation_rstep : forall m1 m2 ths1 ths2 tid e ad,
   ad < #m1 ->
   m1[ad].R = m2[ad].R.
 Proof.
-  intros. invc_ostep; eauto using mreg_preservation_cstep.
+  intros. invc_rstep; eauto using mreg_preservation_cstep.
   repeat omicron; upsilon; eauto using mreg_preservation_cstep;
   invc_cstep; invc_mstep; sigma; auto.
 Qed.
