NoRef.v
@@ -5,56 +5,61 @@ From Elo Require Import Core.
 (* ------------------------------------------------------------------------- *)
 
 Inductive no_ref (ad : addr) : tm -> Prop :=
-  | noref_unit  :                 no_ref ad <{unit          }>
-  | noref_nat   : forall n,       no_ref ad <{nat n         }>
-  | noref_seq   : forall t1 t2,   no_ref ad t1 ->
-                                  no_ref ad t2 ->
-                                  no_ref ad <{t1; t2        }>
-  | noref_var   : forall x,       no_ref ad <{var x         }>
-  | noref_fun   : forall x Tx t,  no_ref ad t  ->
-                                  no_ref ad <{fn x Tx t     }>
-  | noref_call  : forall t1 t2,   no_ref ad t1 ->
-                                  no_ref ad t2 ->
-                                  no_ref ad <{call t1 t2    }>
-  | noref_ref   : forall ad' T,   ad <> ad'    ->
-                                  no_ref ad <{&ad' : T      }>
-  | noref_new   : forall t T,     no_ref ad t  ->
-                                  no_ref ad <{new t : T     }>
-  | noref_init  : forall ad' t T, no_ref ad t  ->
-                                  no_ref ad <{init ad' t : T}>
-  | noref_load  : forall t,       no_ref ad t  ->
-                                  no_ref ad <{*t            }>
-  | noref_asg   : forall t1 t2,   no_ref ad t1 ->
-                                  no_ref ad t2 ->
-                                  no_ref ad <{t1 := t2      }>
-  | noref_acq   : forall t1 x t2, no_ref ad t1 ->
-                                  no_ref ad t2 ->
-                                  no_ref ad <{acq t1 x t2   }>
-  | noref_cr    : forall ad' t,   no_ref ad t  ->
-                                  no_ref ad <{cr ad' t      }>
-  | noref_spawn : forall t,       no_ref ad t ->
-                                  no_ref ad <{spawn t       }>
+  | noref_unit  :                  no_ref ad <{unit                     }>
+  | noref_nat   : forall n,        no_ref ad <{nat n                    }>
+  | noref_seq   : forall t1 t2,    no_ref ad t1 ->
+                                   no_ref ad t2 ->
+                                   no_ref ad <{t1; t2                   }>
+  | noref_if    : forall t1 t2 t3, no_ref ad t1 ->
+                                   no_ref ad t2 ->
+                                   no_ref ad t3 ->
+                                   no_ref ad <{if t1 then t2 else t3 end}>
+  | noref_var   : forall x,        no_ref ad <{var x                    }>
+  | noref_fun   : forall x Tx t,   no_ref ad t  ->
+                                   no_ref ad <{fn x Tx t                }>
+  | noref_call  : forall t1 t2,    no_ref ad t1 ->
+                                   no_ref ad t2 ->
+                                   no_ref ad <{call t1 t2               }>
+  | noref_ref   : forall ad' T,    ad <> ad'    ->
+                                   no_ref ad <{&ad' : T                 }>
+  | noref_new   : forall t T,      no_ref ad t  ->
+                                   no_ref ad <{new t : T                }>
+  | noref_init  : forall ad' t T,  no_ref ad t  ->
+                                   no_ref ad <{init ad' t : T           }>
+  | noref_load  : forall t,        no_ref ad t  ->
+                                   no_ref ad <{*t                       }>
+  | noref_asg   : forall t1 t2,    no_ref ad t1 ->
+                                   no_ref ad t2 ->
+                                   no_ref ad <{t1 := t2                 }>
+  | noref_acq   : forall t1 x t2,  no_ref ad t1 ->
+                                   no_ref ad t2 ->
+                                   no_ref ad <{acq t1 x t2              }>
+  | noref_cr    : forall ad' t,    no_ref ad t  ->
+                                   no_ref ad <{cr ad' t                 }>
+  | noref_spawn : forall t,        no_ref ad t ->
+                                   no_ref ad <{spawn t                  }>
   .
 
 (* inversion --------------------------------------------------------------- *)
 
 Local Ltac _noref tt :=
   match goal with
-  | H : no_ref _   <{unit        }> |- _ => clear H
-  | H : no_ref _   <{nat _       }> |- _ => clear H
-  | H : no_ref _   <{_; _        }> |- _ => tt H
-  | H : no_ref _   <{var _       }> |- _ => clear H
-  | H : no_ref _   <{fn _ _ _    }> |- _ => tt H
-  | H : no_ref _   <{call _ _    }> |- _ => tt H
-  | H : no_ref ?ad <{& ?ad : _   }> |- _ => invc H; auto
-  | H : no_ref _   <{&_ : _      }> |- _ => tt H
-  | H : no_ref _   <{new _ : _   }> |- _ => tt H
-  | H : no_ref _   <{init _ _ : _}> |- _ => tt H
-  | H : no_ref _   <{* _         }> |- _ => tt H
-  | H : no_ref _   <{_ := _      }> |- _ => tt H
-  | H : no_ref _   <{acq _ _ _   }> |- _ => tt H
-  | H : no_ref _   <{cr _ _      }> |- _ => tt H
-  | H : no_ref _   <{spawn _     }> |- _ => tt H
+  | H : no_ref _   <{unit                  }> |- _ => clear H
+  | H : no_ref _   <{nat _                 }> |- _ => clear H
+  | H : no_ref _   <{_; _                  }> |- _ => tt H
+  | H : no_ref _   <{if _ then _ else _ end}> |- _ => tt H
+  | H : no_ref _   <{var _                 }> |- _ => clear H
+  | H : no_ref _   <{fn _ _ _              }> |- _ => tt H
+  | H : no_ref _   <{call _ _              }> |- _ => tt H
+  | H : no_ref ?ad <{& ?ad : _             }> |- _ => invc H; auto
+  | H : no_ref _   <{&_ : _                }> |- _ => tt H
+  | H : no_ref _   <{new _ : _             }> |- _ => tt H
+  | H : no_ref _   <{init _ _ : _          }> |- _ => tt H
+  | H : no_ref _   <{* _                   }> |- _ => tt H
+  | H : no_ref _   <{_ := _                }> |- _ => tt H
+  | H : no_ref _   <{acq _ _ _             }> |- _ => tt H
+  | H : no_ref _   <{cr _ _                }> |- _ => tt H
+  | H : no_ref _   <{spawn _               }> |- _ => tt H
   end.
 
 Ltac inv_noref  := _noref inv.
@@ -178,10 +183,14 @@ Definition no_refs (t : tm) := forall ad, no_ref ad t.
 (* inversion --------------------------------------------------------------- *)
 
 Local Ltac solve_inv_norefs :=
-  unfold no_refs; intros; try split; intros; spec; invc_noref; auto.
+  unfold no_refs; intros; repeat split; intros; spec; invc_noref; auto.
 
 Local Lemma inv_norefs_seq : forall t1 t2,
   no_refs <{t1; t2}> -> no_refs t1 /\ no_refs t2.
+Proof. solve_inv_norefs. Qed.
+
+Local Lemma inv_norefs_if : forall t1 t2 t3,
+  no_refs (tm_if t1 t2 t3) -> no_refs t1 /\ no_refs t2 /\ no_refs t3.
 Proof. solve_inv_norefs. Qed.
 
 Local Lemma inv_norefs_fun : forall x Tx t,
@@ -228,7 +237,8 @@ Ltac invc_norefs :=
   match goal with
   | H : no_refs <{unit        }> |- _ => clear H
   | H : no_refs <{nat _       }> |- _ => clear H
-  | H : no_refs <{_; _        }> |- _ => eapply inv_norefs_seq   in H as [? ?]
+  | H : no_refs <{_; _        }> |- _ => eapply inv_norefs_seq in H as [? ?]
+  | H : no_refs (tm_if _ _ _  )  |- _ => eapply inv_norefs_if  in H as [? [? ?]]
   | H : no_refs <{var _       }> |- _ => clear H
   | H : no_refs <{fn _ _ _    }> |- _ => eapply inv_norefs_fun   in H
   | H : no_refs <{call _ _    }> |- _ => eapply inv_norefs_call  in H as [? ?]
