UniqueInits.v
@@ -259,7 +259,7 @@ Theorem ui_preservation_rstep : forall m1 m2 ths1 ths2 tid e,
   m1 / ths1 ~~~[tid, e]~~> m2 / ths2 ->
   unique_initializers m2 ths2.
 Proof.
-  intros. invc_ostep; eauto using ui_preservation_cstep.
+  intros. invc_rstep; eauto using ui_preservation_cstep.
   match goal with _ : _ / _ ~~[_, _]~~> ?m / ?ths |- _ =>
     assert (unique_initializers m ths)
   end;
@@ -269,9 +269,9 @@ Qed.
 Theorem ui_preservation_base : forall t,
   no_inits t ->
   (* --- *)
-  unique_initializers base_m (base_t t).
+  unique_initializers nil (base t).
 Proof.
-  unfold base_m, base_t. intros ** ? ?. split; intros Hnil.
+  unfold base. intros ** ? ?. split; intros Hnil.
   - intros ad'. simpl in Hnil. destruct ad; upsilon; auto.
   - simpl in Hnil. destruct ad; upsilon; simpl in *; lia.
 Qed.
